powerset construction (different approach using sets)

FormaleSystemeInLean/LectureAndExercise/lecture4.lean
@@ -13,7 +13,7 @@ structure NFA (Q : Type u) (Sigma : Type v) [Fintype Q] [Fintype Sigma] where
   Q0 : List Q
   F : List Q
 
-variable {Q : Type u} {Sigma : Type v} [Fintype Q] [Fintype Sigma] [Fintype (Option Q)] [BEq Q]
+variable {Q : Type u} {Sigma : Type v} [Fintype Q] [Fintype Sigma] [Fintype (Option Q)] [BEq Q] [BEq (Set Q)] [DecidableEq Q] [Fintype (Set Q)]
 
 def NFA.δ_word (nfa : NFA Q Sigma) (R : List Q) : (Word Sigma) → List Q
   | .nil => R
@@ -92,6 +92,23 @@ theorem acc_run_iff_δ_word_contains_final (nfa : NFA Q Sigma) (w : Word Sigma) 
     rcases run with ⟨q0, r, q0_mem⟩
     exists q0, qf, r
 
+
+def Powertype (α : Type u) := Set α
+
+def List.power (l : List α) : List (List α) := sorry -- powerset but defined on lists
+
+def List.toSet (l : List α) : Set α := fun e => e ∈ l
+
+def Set.elem (S : Set α) (a : α) : Bool :=
+  sorry--if a ∈ S then true else false
+
+def Set.toList (S : Set α) [Fintype α] : List α :=
+  Fintype.elems.filter (fun x => S.elem x)
+
+instance (α : Type u) [Fintype α] : Fintype (Powertype α) where
+  elems := Fintype.elems.power.map (List.toSet)
+  complete := by sorry
+
 def DFA.to_NFA (M : DFA Q Sigma) : NFA Q Sigma where
   δ := fun q a =>
     match M.δ q a with
@@ -100,17 +117,16 @@ def DFA.to_NFA (M : DFA Q Sigma) : NFA Q Sigma where
   Q0 := [M.q0]
   F := M.F
 
-def reachable_from (M : NFA Q Sigma) (_ : List Q) (a : Sigma) : List Q  → List Q
-  | .nil => .nil
-  | .cons q R => (q::R.flatMap (fun q => M.δ q a)).eraseDups
+def NFA.to_DFA (M : NFA Q Sigma) : DFA (Powertype Q) Sigma where
+  δ := fun R a => some (R.toList.flatMap (fun q => M.δ q a)).toSet
+  q0 := M.Q0.toSet
+  F := Fintype.elems.filter (fun x => M.F.toSet ∩ x != ∅)
 
-
-variable {Q' : Type u} {T : Fintype Q'} {Φ : @Power Q' T} [BEq Q'] [Fintype (@Power Q' T)] [Fintype (List Q')]
-
-def NFA.to_DFA (M : NFA Q' Sigma) [Fintype (List Q)] : DFA (List Q') Sigma where
-  δ := fun R a => (R.flatMap (fun q => M.δ q a)).eraseDups
-  q0 := M.Q0
-  F := Φ.elems.filter (fun x => x.any (M.F.contains · ))
+-- geht es auch so? Eigentlic müsste ja sowieso ein totaler DFA rauskommen. Außerdem wissen wir ja L(DFA_total) = L(DFA)
+def NFA.to_TotalDFA (M : NFA Q Sigma) : TotalDFA (Powertype Q) Sigma where
+  δ := fun R a => (R.toList.flatMap (fun q => M.δ q a)).toSet
+  q0 := M.Q0.toSet
+  F := Fintype.elems.filter (fun x => M.F.toSet ∩ x != ∅)
 
 theorem to_NFA_lang_eq (M : DFA Q Sigma) : M.to_NFA.Language = M.Language := by
   apply Set.ext
@@ -143,3 +159,70 @@ theorem to_NFA_lang_eq (M : DFA Q Sigma) : M.to_NFA.Language = M.Language := by
     .
       sorry
     . sorry
+
+theorem δ_powersetDFA_eq_some (M : NFA Q Sigma) (a : Sigma) (R : Powertype Q) : M.to_DFA.δ R a ≠ none := by
+  unfold NFA.to_DFA
+  grind
+
+theorem δ_word_powersetDFA_eq_some (M : NFA Q Sigma) (w : Word Sigma) (R : Powertype Q) : M.to_DFA.δ_word R w ≠ none := by
+  unfold DFA.δ_word
+  by_cases h : w = []
+  . simp only [h]
+    apply Option.some_ne_none
+  . rw [← Ne.eq_1, List.ne_nil_iff_exists_cons] at h
+    rcases h with ⟨a, v, w_eq⟩
+    simp only [w_eq, NFA.to_DFA]
+
+
+    sorry
+
+theorem δ_NFA_subset_δ_powersetDFA (M : NFA Q Sigma) (a : Sigma) (R : Powertype Q) : q ∈ R.toList → (M.δ q a).toSet ⊆ M.to_TotalDFA.δ R a := by
+  intro q_mem
+  intro q' q'_mem
+  simp only [NFA.to_TotalDFA]
+  unfold List.toSet at *
+  simp only [Membership.mem] at *
+  apply List.mem_flatMap_of_mem q_mem
+  exact q'_mem
+
+theorem δ_NFA_eq_δ_TotalDFA (M : NFA Q Sigma) (a : Sigma) (R : List Q) : M.to_TotalDFA.δ R.toSet a = (M.δ_word R [a]).toSet := by
+  simp only [NFA.to_TotalDFA, NFA.δ_word]
+  apply congrArg -- ARRRGGG indeed
+
+  sorry
+
+theorem δ_word_eq_DFA_NFA (M : NFA Q Sigma) (w : Word Sigma) (R : List Q) [Inhabited (Powertype Q)] [BEq (Powertype Q)] : (M.δ_word R w).toSet = M.to_TotalDFA.δ_word R.toSet w := by
+  apply Set.ext
+  intro q
+  constructor
+  . intro q_mem
+    induction w generalizing q R with
+    | nil =>
+      unfold NFA.δ_word at q_mem
+      grind
+    | cons a v ih =>
+      simp only [NFA.δ_word] at q_mem
+      have aux := ih (List.flatMap (fun x => M.δ x a) R) q q_mem
+      simp only [TotalDFA.δ_word]
+      --unfold List.toSet at *
+      --simp only [Membership.mem] at *
+      sorry
+  . sorry
+
+theorem to_DFA_lang_eq (M : NFA Q Sigma) : M.to_DFA.Language = M.Language := by
+  apply Set.ext
+  intro w
+  constructor
+  . intro w_mem
+    --rw [acc_run_iff_δ_word_contains_final]
+    unfold DFA.Language at w_mem
+    simp only [Membership.mem] at w_mem
+    rcases w_mem with ⟨q, d_eq, q_mem⟩
+    simp only [NFA.Language, Membership.mem]
+    sorry
+  . sorry
+
+
+
+
+-- ++++++++++++++++++++++++++++++++++++++++++++++++++++++++++++++++++++++++++++++++++++++++++++++++++++++++++++++++++++++++++++++++++++++++++++++++++++++++++++++++++++++++++++++++++++++++++++++++++++++
