FormaleSystemeInLean/LectureAndExercise/temporary_defs.lean
@@ -1,0 +1,327 @@
+import FormaleSystemeInLean.LectureAndExercise.lecture1
+
+set_option linter.unusedSectionVars false
+
+-- inspired by mathlib
+class Fintype (α : Type u) where
+  elems : List α
+  complete : ∀ a : α, a ∈ elems
+
+def List.toSet (l : List α) : Set α := fun e => e ∈ l
+
+def Set.map (f : α → β) (S : Set α) [DecidablePred S] [Fintype α] : Set β :=
+  ((Fintype.elems.filter (· ∈ S)).map (fun x => f x)).toSet
+
+def Set.toList (S : Set α) [DecidablePred S] [Fintype α] : List α :=
+  Fintype.elems.filter (· ∈ S)
+
+theorem Set.mem_map (f : α → β) (S : Set α) (b : β) [DecidablePred S] [Fintype α] : b ∈ Set.map f S ↔ ∃ a, a ∈ S ∧ f a = b := by
+  simp only [Set.map]
+  constructor
+  . intro h
+    rcases List.mem_map.mp h with ⟨a, a_mem_f, rfl⟩
+    rcases List.mem_filter.mp a_mem_f with ⟨a_mem, ha_S⟩
+    sorry
+  . intro h
+    rcases h with ⟨a, a_mem, fa_eq⟩
+    unfold List.toSet
+    simp only [Membership.mem]
+
+    sorry
+
+structure DFA (Q : Type u) (Sigma : Type v) [Fintype Q] where
+  𝓠 : Set Q
+  δ : Q → Sigma → Option Q
+  q0 : Q
+  F : Set Q
+
+structure TotalDFA (Q : Type u) (Sigma : Type v) [Fintype Q] where
+  𝓠 : Set Q
+  δ : Q → Sigma → Q
+  q0 : Q
+  F : Set Q
+
+structure NFA (Q : Type u) (Sigma : Type v) [Fintype Q] [Fintype Sigma] [Fintype (Set Q)] where
+  𝓠: Set Q
+  δ: Q -> Sigma → Set Q
+  Q0 : Set Q
+  F : Set Q
+
+variable {Q : Type u} {Sigma : Type v} [Fintype Q] [Fintype Sigma] [Fintype (Option Q)] [BEq Q] [BEq (Set Q)] [DecidableEq Q] [Fintype (Set Q)]
+
+def DFA.δ_word (dfa : DFA Q Sigma) (q : Q) : (Word Sigma) -> Option Q
+| .nil => .some q
+| .cons a v => (dfa.δ q a).bind (fun q' => dfa.δ_word q' v)
+
+def TotalDFA.δ_word (dfa : TotalDFA Q Sigma) (q : Q) : (Word Sigma) -> Q
+  | .nil => q
+  | .cons a v => dfa.δ_word (dfa.δ q a) v
+
+def NFA.δ_word (nfa : NFA Q Sigma) (R : Set Q) : (Word Sigma) → Set Q
+  | .nil => R
+  | .cons a v => nfa.δ_word (fun q' => ∃ q, q ∈ R ∧ q' ∈ nfa.δ q a ) v
+
+def DFA.Language (dfa : DFA Q Sigma) : Language Sigma :=
+  fun w => ∃ qf, dfa.δ_word dfa.q0 w = some qf ∧ qf ∈ dfa.F
+
+def DFA.to_totalDFA (M : DFA Q Sigma) [DecidablePred M.F] [DecidablePred M.𝓠] : TotalDFA (Option Q) Sigma where
+  𝓠 := M.𝓠.map fun q => some q
+  δ := fun q a => q.bind (M.δ · a)
+  q0 := .some M.q0
+  F := M.F.map fun q => some q
+
+def TotalDFA.Language (dfa : TotalDFA Q Sigma) : Language Sigma :=
+  fun w => dfa.δ_word dfa.q0 w ∈ dfa.F
+
+inductive NFA.Run (nfa : NFA Q Sigma) : Q -> Q -> Word Sigma -> Type _
+| self (q : Q) : nfa.Run q q []
+| step {q1 q2 qf : Q} {a : Sigma} {v : Word Sigma} (r : nfa.Run q2 qf v) (q2_mem : q2 ∈ nfa.δ q1 a) : nfa.Run q1 qf (a :: v)
+
+def NFA.Run.from_start {nfa : NFA Q Sigma} (_ : nfa.Run q0 q w) : Prop := q0 ∈ nfa.Q0
+def NFA.Run.accepts {nfa : NFA Q Sigma} (_ : nfa.Run q qf w) : Prop := qf ∈ nfa.F
+
+def NFA.Language (nfa : NFA Q Sigma) : Language Sigma :=
+  fun w => ∃ (q0 qf : Q) (r : nfa.Run q0 qf w), r.from_start ∧ r.accepts
+
+def NFA.to_TotalDFA (M : NFA Q Sigma) : TotalDFA (Set Q) Sigma where
+  𝓠 := M.𝓠.powerset
+  δ := fun R a => fun q' => ∃ q, q ∈ R ∧ q' ∈ M.δ q a
+  q0 := M.Q0
+  F := fun R => ∃ q ∈ R, q ∈ M.F
+
+--+++++++++++++++++++++++++++++++++++++++++++++++++++++++++++++++++++++++++++++++++++++++++++++++++++++++
+-- TotalDFA Theorems
+
+theorem final_iff_final (M : DFA Q Sigma) (q : Q) [DecidablePred M.F] [DecidablePred M.𝓠]  : q ∈ M.F ↔ some q ∈ M.to_totalDFA.F := by
+  constructor
+  . intro q_mem
+    unfold DFA.to_totalDFA
+    simp only [Set.mem_map]
+    exists q
+  . intro q_mem
+    unfold DFA.to_totalDFA at q_mem
+    simp only [Set.mem_map] at q_mem
+    rcases q_mem with ⟨q', q'_mem, sqf_eq⟩
+    rw [Option.some_inj] at sqf_eq
+    rw [← sqf_eq]
+    exact q'_mem
+
+theorem δ_eq_δ (M : DFA Q Sigma) (q : Q) (a : Sigma) [DecidablePred M.F] [DecidablePred M.𝓠]  : M.δ q a = M.to_totalDFA.δ q a := by
+  unfold DFA.to_totalDFA
+  simp
+
+theorem δ_none_eq_none (M : DFA Q Sigma) (a : Sigma) [DecidablePred M.F] [DecidablePred M.𝓠]  : M.to_totalDFA.δ none a = none := by
+  trivial -- to do: ohne trivial???
+
+theorem garbage_state (M : DFA Q Sigma) (w : Word Sigma) [DecidablePred M.F] [DecidablePred M.𝓠]  : M.to_totalDFA.δ_word none w = none := by
+  induction w with
+  | nil =>
+    trivial
+  | cons a v ih =>
+    unfold TotalDFA.δ_word
+    rw [δ_none_eq_none]
+    exact ih
+
+theorem final_ne_none (M : DFA Q Sigma) [DecidablePred M.F] [DecidablePred M.𝓠] : q ∈ M.to_totalDFA.F → q ≠ none := by
+  intro q_mem
+  simp only [DFA.to_totalDFA] at q_mem
+  rw [Set.mem_map] at q_mem
+  rcases q_mem with ⟨q', a, b⟩
+  rw [←b]
+  apply Option.some_ne_none
+
+theorem δ_word_eq_δ_word (M : DFA Q Sigma) (q : Q) (w : Word Sigma) [DecidablePred M.F] [DecidablePred M.𝓠] : M.δ_word q w = M.to_totalDFA.δ_word q w := by
+  induction w generalizing q with
+  | nil =>
+    trivial
+  | cons a v ih =>
+    rw [DFA.δ_word, TotalDFA.δ_word]
+    simp only [δ_eq_δ]
+    cases hd : M.to_totalDFA.δ (some q) a with
+    | none =>
+      simp only [Option.bind]
+      unfold TotalDFA.δ_word
+      cases hv : v with
+      | nil =>
+        simp
+      | cons a' v' =>
+        simp only [hv]
+        rw [δ_none_eq_none]
+        rw [garbage_state]
+    | some q' =>
+      apply ih
+
+theorem totalDFA_eq_DFA (M : DFA Q Sigma) [DecidablePred M.F] [DecidablePred M.𝓠] : M.Language = (M.to_totalDFA).Language := by
+  apply Set.ext
+  intro w
+  unfold TotalDFA.Language DFA.Language
+  constructor
+  . intro w_mem
+    rcases w_mem with ⟨qf, w_acc, qf_mem⟩
+    rw [δ_word_eq_δ_word] at w_acc
+    rw [final_iff_final] at qf_mem
+    have aux : M.to_totalDFA.q0 = some M.q0 := by simp only [DFA.to_totalDFA]
+    simp only [Membership.mem, aux]
+    rw [w_acc]
+    exact qf_mem
+  . intro w_mem
+    have aux : ∃ qf, M.to_totalDFA.δ_word M.to_totalDFA.q0 w = some qf := by
+      rw [← Option.isSome_iff_exists, Option.isSome_iff_ne_none]
+      simp only [Membership.mem] at w_mem
+      apply final_ne_none (Sigma := Sigma) (M := M) (q := M.to_totalDFA.δ_word M.to_totalDFA.q0 w)
+      exact w_mem
+    rcases aux with ⟨qf, qf_eq⟩
+    exists qf
+    constructor
+    . rw [δ_word_eq_δ_word]
+      exact qf_eq
+    . simp only [DFA.to_totalDFA, Set.mem_map] at w_mem
+      rcases w_mem with ⟨qf', qf'_mem, qf'_eq⟩
+      simp only [DFA.to_totalDFA] at qf_eq
+      rw [qf_eq, Option.some_inj] at qf'_eq
+      rw [← qf'_eq]
+      exact qf'_mem
+
+--+++++++++++++++++++++++++++++++++++++++++++++++++++++++++++++++++++++++++++++++++++++++++++++++++++++++++
+-- NFA theorems
+
+-- for every run q1...qn on a word w with q1 ∈ R, qn ∈ δ_word(R, w).
+theorem run_imp_mem_δ (nfa : NFA Q Sigma) (q1 qn : Q) (R : Set Q) (w : Word Sigma) : nfa.Run q1 qn w → q1 ∈ R → qn ∈ nfa.δ_word R w := by
+  intro r q1_mem
+  induction r generalizing R with
+  | self q =>
+    trivial
+  | @step qa qb qc a v r qb_mem hr =>
+    have aux : qc ∈ nfa.δ_word (nfa.δ qa a) v := hr (nfa.δ qa a) qb_mem
+    unfold NFA.δ_word
+    let Z : Set Q := fun q' => ∃ q, q ∈ R ∧ q' ∈ nfa.δ q a
+    have aux2 : ∀ q, q ∈ nfa.δ qa a → q ∈ Z := by
+      intro q q_mem
+      simp only [Z, Membership.mem]
+      exists qa
+    grind
+
+-- given a set of states R and a state qn ∈ δ(R, w) we can also construct a run for w starting with a state in R.
+theorem run_from_δ_word (nfa : NFA Q Sigma) (qn : Q) (R : Set Q) (w : Word Sigma) : qn ∈ nfa.δ_word R w → ∃ (q1 : Q) (_ : nfa.Run q1 qn w), q1 ∈ R := by
+  intro qn_mem
+  induction w generalizing R with
+  | nil =>
+    simp only [Membership.mem] at qn_mem
+    unfold NFA.δ_word at qn_mem
+    exists qn
+    exists NFA.Run.self qn
+  | cons a v ih =>
+    simp only [Membership.mem, NFA.δ_word] at qn_mem
+    let Z : Set Q := fun q' => ∃ q, R q ∧ nfa.δ q a q'
+    have aux := ih Z qn_mem
+    rcases aux with ⟨q, r', q_mem⟩
+    have aux2 : ∃ q', q' ∈ R ∧ q ∈ nfa.δ q' a := by
+      rcases q_mem with ⟨q', q'_mem, q_mem⟩
+      exists q'
+    rcases aux2 with ⟨q', q'_mem, q'_memd⟩
+    exists q'
+    exists NFA.Run.step r' q'_memd
+
+-- Using the two previous results, we can show that the two different definitions for the language accepted by an NFA are equal:
+-- An NFA has an accepting run q0...qf on a word w iff the set of states reachable from q0 ∈ Q0 contains a qf ∈ F.
+theorem acc_run_iff_δ_word_contains_final (nfa : NFA Q Sigma) (w : Word Sigma) : w ∈ nfa.Language ↔ ∃ q ∈ nfa.δ_word nfa.Q0 w, q ∈ nfa.F := by
+  constructor
+  . intro w_mem
+    rcases w_mem with ⟨q0, qf, r, r_s, r_acc⟩
+    unfold NFA.Run.accepts at r_acc
+    unfold NFA.Run.from_start at r_s
+    have qf_mem : qf ∈ nfa.δ_word nfa.Q0 w := run_imp_mem_δ nfa q0 qf nfa.Q0 w r r_s
+    exists qf
+  . intro h
+    unfold NFA.Language
+    simp only [Membership.mem]
+    rcases h with ⟨qf, q_memd, q_memf⟩
+    have run := run_from_δ_word nfa qf nfa.Q0 w q_memd
+    rcases run with ⟨q0, r, q0_mem⟩
+    exists q0, qf, r
+
+theorem δ_NFA_eq_δ_TotalDFA (M : NFA Q Sigma) (a : Sigma) (R : Set Q) : M.to_TotalDFA.δ R a = M.δ_word R [a] := by
+  simp only [NFA.to_TotalDFA, NFA.δ_word]
+
+ theorem δ_word_eq_DFA_NFA (M : NFA Q Sigma) (w : Word Sigma) (R : Set Q): M.δ_word R w = M.to_TotalDFA.δ_word R w := by
+  induction w generalizing R with
+  | nil =>
+    simp only [NFA.δ_word, TotalDFA.δ_word]
+  | cons a v ih =>
+    simp only [NFA.δ_word, TotalDFA.δ_word]
+    grind -- warum
+
+theorem to_DFA_lang_eq (M : NFA Q Sigma) : M.to_TotalDFA.Language = M.Language := by
+  apply Set.ext
+  intro w
+  unfold TotalDFA.Language
+  constructor
+  . intro w_mem
+    rw [acc_run_iff_δ_word_contains_final]
+    simp only [Membership.mem] at *
+    cases w with
+    | nil =>
+      simp only [TotalDFA.δ_word, NFA.to_TotalDFA] at w_mem
+      rcases w_mem with ⟨q0, q0_mems, q0_memf⟩
+      exists q0
+    | cons a v =>
+      rcases w_mem with ⟨q, q_memd, q_memf⟩
+      exists q
+      rw [δ_word_eq_DFA_NFA]
+      constructor
+      . exact q_memd
+      . exact q_memf
+  . intro w_mem
+    rw [acc_run_iff_δ_word_contains_final] at w_mem
+    simp only [Membership.mem]
+    rcases w_mem with ⟨q, q_memd, q_memf⟩
+    cases w with
+    | nil =>
+      unfold NFA.δ_word at q_memd
+      simp only [TotalDFA.δ_word, NFA.to_TotalDFA]
+      exists q
+    | cons a v =>
+      rw [δ_word_eq_DFA_NFA] at q_memd
+      simp only [TotalDFA.δ_word, NFA.to_TotalDFA]
+      exists q
+
+def DFA.to_NFA (M : DFA Q Sigma) : NFA Q Sigma where
+  𝓠 := sorry
+  δ := fun q a =>
+    match M.δ q a with
+    | none => ∅
+    | some q => fun q => q = q
+  Q0 := fun q => q = M.q0
+  F := M.F
+
+theorem to_NFA_lang_eq (M : DFA Q Sigma) : M.to_NFA.Language = M.Language := by
+  apply Set.ext
+  intro w
+  constructor
+  . intro w_mem
+    simp only [DFA.Language, Membership.mem]
+    rw [acc_run_iff_δ_word_contains_final] at w_mem
+    rcases w_mem with ⟨qf, qf_memd, qf_memf⟩
+    simp only [DFA.to_NFA] at qf_memf
+    exists qf
+    constructor
+    . induction w with
+      | nil =>
+        simp only [NFA.δ_word, DFA.to_NFA, List.mem_singleton] at qf_memd
+        simp only [DFA.δ_word, Option.some_inj]
+        rw [qf_memd]
+      | cons a v ih =>
+        simp only [NFA.δ_word] at qf_memd
+        simp only [DFA.δ_word]
+        sorry
+    . trivial
+  . intro w_mem
+    simp only [DFA.Language, Membership.mem] at w_mem
+    rcases w_mem with ⟨qf, qf_eq, qf_memf⟩
+    unfold DFA.δ_word at qf_eq
+    rw [acc_run_iff_δ_word_contains_final]
+    exists qf
+    constructor
+    .
+      sorry
+    . sorry
